Separated Multisubst out of Termination

03Debruijn/Termination.thy
@@ -1,5 +1,5 @@
 theory Termination
-  imports Debruijn
+  imports Multisubst
 begin
 
 abbreviation terminatesd :: "dexpr \<Rightarrow> bool" where
@@ -10,38 +10,11 @@ primrec stable :: "ty \<Rightarrow> dexpr \<Rightarrow> bool" where
 | "stable (Arrow t\<^sub>1 t\<^sub>2) e = (terminatesd e \<and> ([] \<turnstile>\<^sub>d e : Arrow t\<^sub>1 t\<^sub>2) \<and> 
     (\<forall>e'. stable t\<^sub>1 e' \<longrightarrow> vald e' \<longrightarrow> stable t\<^sub>2 (DApp e e')))"
 
-inductive subst_pairs :: "ty list \<Rightarrow> dexpr list \<Rightarrow> bool" where
-  subp_nil [simp]: "subst_pairs [] []"
-| subp_cons [simp]: "stable t e \<Longrightarrow> vald e \<Longrightarrow> subst_pairs \<Gamma> es \<Longrightarrow> subst_pairs (t # \<Gamma>) (e # es)"
-
-primrec multisubst :: "dexpr list \<Rightarrow> dexpr \<Rightarrow> dexpr" where
-  "multisubst [] e = e"
-| "multisubst (e' # es) e = multisubst es (substd 0 e' e)"
-
 lemma [simp]: "stable t e \<Longrightarrow> [] \<turnstile>\<^sub>d e : t"
   by (induction t) simp_all
 
 lemma [simp]: "stable t e \<Longrightarrow> terminatesd e"
   by (induction t) simp_all
-
-lemma [simp]: "subst_pairs \<Gamma> es \<Longrightarrow> stable t e \<Longrightarrow> vald e \<Longrightarrow> x \<le> length \<Gamma> \<Longrightarrow> 
-  subst_pairs (insert_at x t \<Gamma>) (insert_at x e es)"
-proof (induction \<Gamma> es arbitrary: x rule: subst_pairs.induct)
-  case (subp_cons t' e' \<Gamma> es)
-  then show ?case by (induction x) simp_all
-qed simp_all
-
-lemma [simp]: "subst_pairs \<Gamma> es \<Longrightarrow> \<Gamma> \<turnstile>\<^sub>d e : t \<Longrightarrow> [] \<turnstile>\<^sub>d multisubst es e : t"
-proof (induction \<Gamma> es arbitrary: e rule: subst_pairs.induct)
-  case (subp_cons t' e' \<Gamma> es)
-  moreover from subp_cons have "insert_at 0 t' \<Gamma> \<turnstile>\<^sub>d e : t" by (induction \<Gamma>) simp_all
-  moreover from subp_cons have "[] \<turnstile>\<^sub>d e' : t'" by simp
-  moreover hence "\<Gamma> \<turnstile>\<^sub>d e' : t'" using tc_postpend by fastforce
-  ultimately show ?case by simp
-qed simp_all
-
-lemma [simp]: "[] \<turnstile>\<^sub>d e : t \<Longrightarrow> multisubst es e = e"
-  by (induction es) simp_all
 
 lemma [simp]: "terminatesd (DConst k)"
 proof
@@ -61,76 +34,26 @@ proof (induction es)
   with Cons show ?case by simp
 qed simp_all
 
-lemma [simp]: "subst_pairs \<Gamma> es \<Longrightarrow> lookup \<Gamma> x = Some t \<Longrightarrow> stable t (multisubst es (DVar x))"
+lemma [simp]: "subst_pairs \<Gamma> es \<Longrightarrow> list_all2 stable \<Gamma> es \<Longrightarrow> lookup \<Gamma> x = Some t \<Longrightarrow> 
+  stable t (multisubst es (DVar x))"
 proof (induction \<Gamma> es arbitrary: x rule: subst_pairs.induct)
   case (subp_cons t' e \<Gamma> ves)
   thus ?case by (induction x) simp_all
 qed simp_all
 
-lemma multisubst_var [simp]: "lookup vs x = Some v \<Longrightarrow> 
-    (\<And>v es. v \<in> set vs \<Longrightarrow> multisubst es v = v) \<Longrightarrow> multisubst vs (DVar x) = v"
-  by (induction vs x rule: lookup.induct) simp_all
-
-lemma [simp]: "multisubst es (DConst k) = DConst k"
-  by (induction es) simp_all
-
-lemma [simp]: "\<exists>e'. multisubst es (DLam t e) = DLam t e'"
-  by (induction es arbitrary: e) simp_all
-
-lemma [simp]: "\<exists>e'. multisubst es (DLam t e) = DLam t e' \<and> 
-    (\<forall>e\<^sub>2. (\<forall>ee. substd 0 ee e\<^sub>2 = e\<^sub>2) \<longrightarrow> substd 0 e\<^sub>2 e' = multisubst es (substd 0 e\<^sub>2 e))"
-  by (induction es arbitrary: e) simp_all
-
-lemma [simp]: "subst_pairs \<Gamma> es \<Longrightarrow> insert_at 0 t\<^sub>1 \<Gamma> \<turnstile>\<^sub>d e : t\<^sub>2 \<Longrightarrow> 
-  \<exists>e'. multisubst es (DLam t\<^sub>1 e) = DLam t\<^sub>1 e' \<and> ([t\<^sub>1] \<turnstile>\<^sub>d e' : t\<^sub>2) \<and>
-    (\<forall>e\<^sub>2. ([] \<turnstile>\<^sub>d e\<^sub>2 : t\<^sub>1) \<longrightarrow> multisubst (insert_at 0 e\<^sub>2 es) e = substd 0 e\<^sub>2 e')"
-proof (induction \<Gamma> es arbitrary: e rule: subst_pairs.induct)
-  case (subp_cons t e' \<Gamma> es)
-  hence "[] \<turnstile>\<^sub>d e' : t" by simp
-  hence "\<Gamma> \<turnstile>\<^sub>d e' : t" using tc_postpend by fastforce
-  hence "insert_at 0 t\<^sub>1 \<Gamma> \<turnstile>\<^sub>d incrd 0 e' : t" by simp
-  with subp_cons have "insert_at 0 t\<^sub>1 \<Gamma> \<turnstile>\<^sub>d substd (Suc 0) (incrd 0 e') e : t\<^sub>2" 
-    by (induction \<Gamma>) simp_all
-  with subp_cons obtain ee' where E: "([t\<^sub>1] \<turnstile>\<^sub>d ee' : t\<^sub>2) \<and> 
-    multisubst es (DLam t\<^sub>1 (substd (Suc 0) (incrd 0 e') e)) = DLam t\<^sub>1 ee' \<and> 
-      (\<forall>e\<^sub>2. ([] \<turnstile>\<^sub>d e\<^sub>2 : t\<^sub>1) \<longrightarrow> 
-        multisubst (insert_at 0 e\<^sub>2 es) (substd (Suc 0) (incrd 0 e') e) = substd 0 e\<^sub>2 ee')" 
-    by fastforce
-  hence "\<And>e\<^sub>2. [] \<turnstile>\<^sub>d e\<^sub>2 : t\<^sub>1 \<Longrightarrow> 
-    multisubst es (substd 0 e\<^sub>2 (substd (Suc 0) (incrd 0 e') e)) = substd 0 e\<^sub>2 ee'" 
-      by (induction es) simp_all
-  hence "\<And>e\<^sub>2. [] \<turnstile>\<^sub>d e\<^sub>2 : t\<^sub>1 \<Longrightarrow> multisubst es (substd 0 e' (substd 0 e\<^sub>2 e)) = substd 0 e\<^sub>2 ee'"
-    by fastforce
-  with E show ?case by simp
-qed simp_all
-
-lemma [simp]: "multisubst es (DApp e\<^sub>1 e\<^sub>2) = DApp (multisubst es e\<^sub>1) (multisubst es e\<^sub>2)"
-  by (induction es arbitrary: e\<^sub>1 e\<^sub>2) simp_all
-
-lemma multisubst_val [simp]: "vald (multisubst es e) \<Longrightarrow> (\<And>e'. e' \<in> set es \<Longrightarrow> vald e') \<Longrightarrow> 
-  vald e \<or> (\<exists>x. e = DVar x \<and> x < length es)"
-proof (induction es arbitrary: e)
-  case (Cons e' es)
-  thus ?case
-  proof (cases "vald (substd 0 e' e)")
-    case True
-    with Cons have "vald e \<or> e = DVar 0" by simp
-    thus ?thesis by fastforce
-  next
-    case False
-    with Cons obtain x where "substd 0 e' e = DVar x \<and> x < length es" by fastforce
-    moreover with Cons have "e = DVar (Suc x)" by fastforce
-    ultimately show ?thesis by simp
-  qed
-qed simp_all
-
-lemma [simp]: "e \<leadsto>\<^sub>d e' \<Longrightarrow> terminatesd e \<Longrightarrow> terminatesd e'"
-proof -
+lemma [simp]: "e \<leadsto>\<^sub>d e' \<Longrightarrow> terminatesd e = terminatesd e'"
+proof 
   assume "terminatesd e"
   then obtain v where V: "vald v \<and> iter (\<leadsto>\<^sub>d) e v" by fastforce
   moreover assume "e \<leadsto>\<^sub>d e'"
   ultimately have "vald v \<and> iter (\<leadsto>\<^sub>d) e' v" by (metis evald_backwards)
-  thus ?thesis by fastforce
+  thus "terminatesd e'" by fastforce
+next
+  assume "terminatesd e'"
+  then obtain v where V: "vald v \<and> iter (\<leadsto>\<^sub>d) e' v" by fastforce
+  moreover assume "e \<leadsto>\<^sub>d e'"
+  ultimately have "vald v \<and> iter (\<leadsto>\<^sub>d) e v" by (metis iter_step)
+  thus "terminatesd e" by fastforce
 qed
 
 lemma stable_evald: "e \<leadsto>\<^sub>d e' \<Longrightarrow> stable t e \<Longrightarrow> stable t e'"
@@ -156,7 +79,9 @@ lemma stable_persists: "iter (\<leadsto>\<^sub>d) e e' \<Longrightarrow> stable 
 lemma stable_evald_back: "[] \<turnstile>\<^sub>d e : t \<Longrightarrow> e \<leadsto>\<^sub>d e' \<Longrightarrow> stable t e' \<Longrightarrow> stable t e"
 proof (induction t arbitrary: e e')
   case Base
-  then show ?case by fastforce
+  from Base(3) have "terminatesd e'" by simp
+  with Base(2) have "terminatesd e" by simp
+  with Base(1) show ?case by simp
 next
   case (Arrow t\<^sub>1 t\<^sub>2)
   from Arrow(5) have "terminatesd e'" by simp
@@ -179,7 +104,8 @@ proof (induction e e' rule: iter.induct)
   thus ?case using stable_evald_back by fastforce
 qed simp_all
 
-lemma tc_stable [simp]: "\<Gamma> \<turnstile>\<^sub>d e : t \<Longrightarrow> subst_pairs \<Gamma> es \<Longrightarrow> stable t (multisubst es e)"
+lemma tc_stable [simp]: "\<Gamma> \<turnstile>\<^sub>d e : t \<Longrightarrow> subst_pairs \<Gamma> es \<Longrightarrow> list_all2 stable \<Gamma> es \<Longrightarrow> 
+  stable t (multisubst es e)"
 proof (induction \<Gamma> e t arbitrary: es rule: typecheckd.induct)
   case (tcd_lam t\<^sub>1 \<Gamma> e t\<^sub>2)
   then obtain e' where E: "multisubst es (DLam t\<^sub>1 e) = DLam t\<^sub>1 e' \<and> ([t\<^sub>1] \<turnstile>\<^sub>d e' : t\<^sub>2) \<and> 
@@ -190,7 +116,8 @@ proof (induction \<Gamma> e t arbitrary: es rule: typecheckd.induct)
     assume S: "stable t\<^sub>1 e\<^sub>2" and V: "vald e\<^sub>2"
     hence E2: "[] \<turnstile>\<^sub>d e\<^sub>2 : t\<^sub>1" by simp
     hence T: "\<exists>t. [] \<turnstile>\<^sub>d e\<^sub>2 : t" by fastforce
-    from tcd_lam have "subst_pairs (insert_at 0 t\<^sub>1 \<Gamma>) (insert_at 0 e\<^sub>2 es) \<Longrightarrow> 
+    from tcd_lam S have "list_all2 stable (insert_at 0 t\<^sub>1 \<Gamma>) (insert_at 0 e\<^sub>2 es)" by simp
+    with tcd_lam have "subst_pairs (insert_at 0 t\<^sub>1 \<Gamma>) (insert_at 0 e\<^sub>2 es) \<Longrightarrow> 
       stable t\<^sub>2 (multisubst (insert_at 0 e\<^sub>2 es) e)" by blast
     with tcd_lam S V T E have "stable t\<^sub>2 (substd 0 e\<^sub>2 e')" by simp
     moreover with V have "DApp (DLam t\<^sub>1 e') e\<^sub>2 \<leadsto>\<^sub>d substd 0 e\<^sub>2 e'" by simp
@@ -225,7 +152,8 @@ qed simp_all
 theorem tc_terminationd [simp]: "[] \<turnstile>\<^sub>d e : t \<Longrightarrow> terminatesd e"
 proof -
   assume "[] \<turnstile>\<^sub>d e : t" 
-  hence "stable t (multisubst [] e)" by (metis subp_nil tc_stable)
+  moreover have "list_all2 stable [] []" by simp
+  ultimately have "stable t (multisubst [] e)" by (metis subp_nil tc_stable)
   thus ?thesis by simp
 qed
 
